---
title: 1.11 Jensen不等式
toc: true
date: 2019-09-16
---

# Jensen不等式

Jensen不等式：对任意凸函数 $f(x)$，有

$$
f(\mathbb{E}(x)) \leqslant \mathbb{E}(f(x))
$$

## 推导

显然，对于任意凸函数，必然有：

$$
f\left(\alpha x_{1}+(1-\alpha) x_{2}\right) \leq \alpha f\left(x_{1}\right)+(1-\alpha) f\left(x_{2}\right)
$$

$$
f(E(x))=f\left(\frac{1}{m} \sum_{i}^{m} x_{i}\right)=f\left(\frac{m-1}{m} \frac{1}{m-1} \sum_{i}^{m-1} x_{i}+\frac{1}{m} x_{i}\right)
$$

取：

$$
\alpha=\frac{m-1}{m}
$$

所以推得：

$$
f(E(x)) \leq \frac{m-1}{m} f\left(\frac{1}{m-1} \sum_{i}^{m-1} x_{i}\right)+\frac{1}{m} f\left(x_{m}\right)
$$

以此类推得：

$$
f(E(x)) \leq \frac{1}{m} f\left(x_{1}\right)+\frac{1}{m} f\left(x_{2}\right)+\ldots \ldots+\frac{1}{m} f\left(x_{m}\right)=E(f(x))
$$



# 相关

- [pumpkin-book](https://github.com/datawhalechina/pumpkin-book)
